lib: Allow additional rules for `datatype_schem`.
Previously, the method `datatype_schem` used a specific list of
hard-coded rules to "fix" datatypes in schematics. This adds an
attribute so users can add new datatype "lenses"/"accessors" as needed.

lib/Monad_WP/Datatype_Schematic.thy
@@ -10,26 +10,48 @@
  *)
 theory Datatype_Schematic
 
-imports Main
-
+imports
+  "../ml-helpers/MLUtils"
+  "../ml-helpers/TermPatternAntiquote"
 begin
 
-text {*
-Introduces a method for improving unification outcomes for
-schematics with datatype expressions as parameters.
+text \<open>
+  Introduces a method for improving unification outcomes for schematics with
+  datatype expressions as parameters.
 
-There are two variants:
-  1. In cases where a schematic is applied to a constant
-like @{term True}, we wrap the constant to avoid some
-undesirable unification candidates.
+  There are two variants:
+    1. In cases where a schematic is applied to a constant like @{term True},
+       we wrap the constant to avoid some undesirable unification candidates.
 
-  2. In cases where a schematic is applied to a constructor expression
-like @{term "Some x"} or @{term "(x, y)"}, we supply selector expressions
-like @{term "the"} or @{term "fst"} to provide more unification candidates.
-This is only done if parameter that would be selected (e.g. @{term x} in
-@{term "Some x"}) contains bound variables which the schematic does not have
-as parameters.
-*}
+    2. In cases where a schematic is applied to a constructor expression like
+       @{term "Some x"} or @{term "(x, y)"}, we supply selector expressions
+       like @{term "the"} or @{term "fst"} to provide more unification
+       candidates.  This is only done if parameter that would be selected (e.g.
+       @{term x} in @{term "Some x"}) contains bound variables which the
+       schematic does not have as parameters.
+
+  In the "constructor expression" case, we let users supply additional
+  constructor handlers via the `datatype_schematic` attribute. The method uses
+  rules of the following form:
+
+    @{term "\<And>x1 x2 x3. getter (constructor x1 x2 x3) = x2"}
+
+  These are essentially simp rules for simple "accessor" primrec functions,
+  which are used to turn schematics like
+
+    @{text "?P (constructor x1 x2 x3)"}
+
+  into
+
+    @{text "?P' x2 (constructor x1 x2 x3)"}.
+\<close>
+
+ML \<open>
+  \<comment> \<open>
+    Anchor used to link error messages back to the documentation above.
+  \<close>
+  val usage_pos = @{here};
+\<close>
 
 definition
   ds_id :: "'a \<Rightarrow> 'a"
@@ -40,8 +62,40 @@ lemma wrap_ds_id:
   "x = ds_id x"
   by (simp add: ds_id_def)
 
-ML {*
+ML \<open>
 structure Datatype_Schematic = struct
+
+fun eq ((idx1, name1, thm1), (idx2, name2, thm2)) =
+  idx1 = idx2 andalso
+  name1 = name2 andalso
+  (Thm.full_prop_of thm1) aconv (Thm.full_prop_of thm2);
+
+structure Datatype_Schematic_Data = Generic_Data
+(
+  \<comment> \<open>
+    Keys are names of datatype constructors (like @{const Cons}), values are
+    `(index, function_name, thm)`.
+
+    - `function_name` is the name of an "accessor" function that accesses part
+      of the constructor specified by the key (so the accessor @{const hd} is
+      related to the constructor/key @{const Cons}).
+
+    - `thm` is a theorem showing that the function accesses one of the
+      arguments to the constructor (like @{thm list.sel(1)}).
+
+    - `idx` is the index of the constructor argument that the accessor
+      accesses.  (eg. since `hd` accesses the first argument, `idx = 0`; since
+      `tl` accesses the second argument, `idx = 1`).
+  \<close>
+  type T = ((int * string * thm) list) Symtab.table;
+  val empty = Symtab.empty;
+  val extend = I;
+  val merge = Symtab.merge_list eq;
+);
+
+fun gen_att m =
+  Thm.declaration_attribute (fn thm => fn context =>
+    Datatype_Schematic_Data.map (m (Context.proof_of context) thm) context);
 
 (* gathers schematic applications from the goal. no effort is made
    to normalise bound variables here, since we'll always be comparing
@@ -55,24 +109,18 @@ fun gather_schem_apps (f $ x) insts = let
     = gather_schem_apps t insts
   | gather_schem_apps _ insts = insts
 
-val actions = Symtab.make_list [
-    (@{const_name Pair}, (0, @{const_name fst}, @{thms prod.sel})),
-    (@{const_name Pair}, (1, @{const_name snd}, @{thms prod.sel})),
-    (@{const_name Some}, (0, @{const_name the}, @{thms option.sel})),
-    (@{const_name Cons}, (0, @{const_name hd}, @{thms list.sel})),
-    (@{const_name Cons}, (1, @{const_name tl}, @{thms list.sel}))]
-
 fun sfirst xs f = get_first f xs
 
-fun get_action prop = let
-    val schem_insts = gather_schem_apps prop []
+fun get_action ctxt prop = let
+    val schem_insts = gather_schem_apps prop [];
+    val actions = Datatype_Schematic_Data.get (Context.Proof ctxt);
     fun mk_sel selname T i = let
         val (argTs, resT) = strip_type T
       in Const (selname, resT --> nth argTs i) end
   in
     sfirst schem_insts
-    (fn (var, xs) => sfirst (xs ~~ (0 upto (length xs - 1)))
-        (try (fn (x, idx) => let
+    (fn (var, xs) => sfirst (Library.tag_list 0 xs)
+        (try (fn (idx, x) => let
             val (c, ys) = strip_comb x
             val (fname, T) = dest_Const c
             val acts = Symtab.lookup_list actions fname
@@ -84,19 +132,19 @@ fun get_action prop = let
           end)))
   end
 
-fun get_bound_tac ctxt = SUBGOAL (fn (t, i) => case get_action t of
-  SOME (Var ((nm, ix), T), idx, sel, thms) => (fn t => let
+fun get_bound_tac ctxt = SUBGOAL (fn (t, i) => case get_action ctxt t of
+  SOME (Var ((nm, ix), T), idx, sel, thm) => (fn t => let
     val (argTs, _) = strip_type T
     val ix2 = Thm.maxidx_of t + 1
     val xs = map (fn (i, T) => Free ("x" ^ string_of_int i, T))
-        (1 upto length argTs ~~ argTs)
+        (Library.tag_list 1 argTs)
     val nx = sel $ nth xs idx
     val v' = Var ((nm, ix2), fastype_of nx --> T)
     val inst_v = fold lambda (rev xs) (betapplys (v' $ nx, xs))
     val t' = Drule.infer_instantiate ctxt
         [((nm, ix), Thm.cterm_of ctxt inst_v)] t
     val t'' = Conv.fconv_rule (Thm.beta_conversion true) t'
-  in safe_full_simp_tac (clear_simpset ctxt addsimps thms) i t'' end)
+  in safe_full_simp_tac (clear_simpset ctxt addsimps [thm]) i t'' end)
   | _ => no_tac)
 
 fun id_applicable (f $ x) = let
@@ -139,25 +187,119 @@ fun wrap_conv ctxt ct = case Thm.term_of ct of
 fun CONVERSION_opt conv i t = CONVERSION conv i t
     handle Option => no_tac t
 
+exception Datatype_Schematic_Error of Pretty.T;
+
+fun apply_pos_markup pos text =
+  let
+    val props = Position.def_properties_of pos;
+    val markup = Markup.properties props (Markup.entity "" "");
+  in Pretty.mark_str (markup, text) end;
+
+fun invalid_accessor ctxt thm : exn =
+  Datatype_Schematic_Error ([
+    Pretty.str "Bad input theorem '",
+    Syntax.pretty_term ctxt (Thm.full_prop_of thm),
+    Pretty.str "'. Click ",
+    apply_pos_markup usage_pos "*here*",
+    Pretty.str " for info on the required rule format." ] |> Pretty.paragraph);
+
+local
+  fun dest_accessor' thm =
+    case (thm |> Thm.full_prop_of |> HOLogic.dest_Trueprop) of
+      @{term_pat "?fun_name ?data_pat = ?rhs"} =>
+        let
+          val fun_name = Term.dest_Const fun_name |> fst;
+          val (data_const, data_args) = Term.strip_comb data_pat;
+          val data_vars = data_args |> map (Term.dest_Var #> fst);
+          val rhs_var = rhs |> Term.dest_Var |> fst;
+          val data_name = Term.dest_Const data_const |> fst;
+          val rhs_idx = ListExtras.find_index (curry op = rhs_var) data_vars |> the;
+        in (fun_name, data_name, rhs_idx) end;
+in
+  fun dest_accessor ctxt thm =
+    case try dest_accessor' thm of
+      SOME x => x
+    | NONE => raise invalid_accessor ctxt thm;
+end
+
+fun add_rule ctxt thm data =
+  let
+    val (fun_name, data_name, idx) = dest_accessor ctxt thm;
+    val entry = (data_name, (idx, fun_name, thm));
+  in Symtab.insert_list eq entry data end;
+
+fun del_rule ctxt thm data =
+  let
+    val (fun_name, data_name, idx) = dest_accessor ctxt thm;
+    val entry = (data_name, (idx, fun_name, thm));
+  in Symtab.remove_list eq entry data end;
+
+val add = gen_att add_rule;
+val del = gen_att del_rule;
+
 fun wrap_tac ctxt = CONVERSION_opt (wrap_conv ctxt)
 
 fun tac1 ctxt = REPEAT_ALL_NEW (get_bound_tac ctxt) THEN' (TRY o wrap_tac ctxt)
 
 fun tac ctxt = tac1 ctxt ORELSE' wrap_tac ctxt
 
-val method
-    = Args.context >> (fn _ => fn ctxt => Method.SIMPLE_METHOD' (tac ctxt));
+val add_section =
+  Args.add -- Args.colon >> K (Method.modifier add @{here});
+
+val method =
+  Method.sections [add_section] >> (fn _ => fn ctxt => Method.SIMPLE_METHOD' (tac ctxt));
 
 end
-*}
+\<close>
 
-method_setup datatype_schem = {* Datatype_Schematic.method *}
+setup \<open>
+  Attrib.setup
+    @{binding "datatype_schematic"}
+    (Attrib.add_del Datatype_Schematic.add Datatype_Schematic.del)
+    "Accessor rules to fix datatypes in schematics"
+\<close>
 
-lemma datatype_schem_demo:
+method_setup datatype_schem = \<open>
+  Datatype_Schematic.method
+\<close>
+
+declare prod.sel[datatype_schematic]
+declare option.sel[datatype_schematic]
+declare list.sel(1,3)[datatype_schematic]
+
+locale datatype_schem_demo begin
+
+lemma handles_nested_constructors:
   "\<exists>f. \<forall>y. f True (Some [x, (y, z)]) = y"
   apply (rule exI, rule allI)
   apply datatype_schem
   apply (rule refl)
   done
+
+datatype foo =
+    basic nat int
+  | another nat
+
+primrec get_basic_0 where
+  "get_basic_0 (basic x0 x1) = x0"
+
+primrec get_nat where
+    "get_nat (basic x _) = x"
+  | "get_nat (another z) = z"
+
+lemma selectively_exposing_datatype_arugments:
+  notes get_basic_0.simps[datatype_schematic]
+  shows "\<exists>x. \<forall>a b. x (basic a b) = a"
+  apply (rule exI, (rule allI)+)
+  apply datatype_schem \<comment> \<open>Only exposes `a` to the schematic.\<close>
+  by (rule refl)
+
+lemma method_handles_primrecs_with_two_constructors:
+  shows "\<exists>x. \<forall>a b. x (basic a b) = a"
+  apply (rule exI, (rule allI)+)
+  apply (datatype_schem add: get_nat.simps)
+  by (rule refl)
+
+end
 
 end
